FoC/Book/Chapter03/Section06.lean
@@ -166,11 +166,31 @@ theorem dfa_state_elimination_regex_complete
     w ∈ RegExp.Denote (RegularLanguage.DFARegex alphabet M) :=
   RegularLanguage.dfaRegex_complete alphabet M halphabet hw
 
+theorem dfa_state_elimination_regex_decidable_sound [DecidableEq state]
+    (alphabet : List alpha) (M : DFA alpha state) [DecidablePred M.accept]
+    {w : Word alpha}
+    (hw : w ∈ RegExp.Denote (RegularLanguage.DFARegexDecidable alphabet M)) :
+    DFA.Accepts M w :=
+  RegularLanguage.dfaRegexDecidable_sound alphabet M hw
+
+theorem dfa_state_elimination_regex_decidable_complete [DecidableEq state]
+    (alphabet : List alpha) (halphabet : forall a, a ∈ alphabet)
+    (M : DFA alpha state) [DecidablePred M.accept] {w : Word alpha}
+    (hw : DFA.Accepts M w) :
+    w ∈ RegExp.Denote (RegularLanguage.DFARegexDecidable alphabet M) :=
+  RegularLanguage.dfaRegexDecidable_complete alphabet M halphabet hw
+
 theorem dfa_recognizable_language_is_regular
     (alphabet : List alpha) (halphabet : forall a, a ∈ alphabet)
     {L : Language alpha} (hL : RegularLanguage.DFARecognizable L) :
     RegularLanguage.Regular L :=
   RegularLanguage.dfa_recognizable_regular alphabet halphabet hL
+
+theorem dfa_language_is_regular_decidable [DecidableEq state]
+    (alphabet : List alpha) (halphabet : forall a, a ∈ alphabet)
+    (M : DFA alpha state) [DecidablePred M.accept] :
+    RegularLanguage.Regular (DFA.Language M) :=
+  RegularLanguage.dfa_language_regular_decidable alphabet halphabet M
 
 theorem nfa_language_is_regular
     (alphabet : List alpha) (halphabet : forall a, a ∈ alphabet)
